continue automation

Hnr.thy
@@ -11,18 +11,62 @@ definition id_assn where "id_assn a c = \<up>(c = a)"
 
 abbreviation array_assn where "array_assn xs xsi \<equiv> xsi \<mapsto>\<^sub>a xs"
 
+named_theorems hnr_rule
+named_theorems hnr_rule_2
+named_theorems hnr_rule_diff_arr
+
 lemma hnr_return: "hnr \<Gamma> (return x) \<Gamma> id_assn x"
   unfolding hnr_def id_assn_def
   by sep_auto
 
-lemma hnr_let:
+lemma keep_drop_1:
+  assumes
+    "\<Gamma>\<^sub>1 \<Longrightarrow>\<^sub>A K\<^sub>1 * D\<^sub>1"
+    "\<Gamma>\<^sub>2 \<Longrightarrow>\<^sub>A K\<^sub>2 * D\<^sub>2"
+  shows 
+    "\<Gamma>\<^sub>1 * \<Gamma>\<^sub>2 \<Longrightarrow>\<^sub>A (K\<^sub>1 * K\<^sub>2) * (D\<^sub>1 * D\<^sub>2)"
+  apply(sep_drule r: assms(1))
+  apply(sep_drule r: assms(2))
+  by sep_auto
+
+lemma keep_drop_2: "A \<Longrightarrow>\<^sub>A A * emp"
+  by sep_auto
+
+lemma keep_drop_3: "A \<Longrightarrow>\<^sub>A emp * A"
+  by sep_auto
+
+lemmas keep_drop_step = keep_drop_1 keep_drop_2 keep_drop_3
+
+definition keep_drop where "keep_drop \<Gamma> K D \<equiv> \<Gamma> \<Longrightarrow>\<^sub>A K * D"
+
+lemma keep_drop_init:
+  assumes
+    "\<Gamma>  \<Longrightarrow>\<^sub>A K' * D'"
+    "K' \<Longrightarrow>\<^sub>A K"
+    "D' \<Longrightarrow>\<^sub>A D"
+  shows
+    "keep_drop \<Gamma> K D"
+  unfolding keep_drop_def
+  using assms(1) assms(2) assms(3) ent_star_mono ent_trans by blast
+
+method keep_drop_simp = (simp only: star_aci)?; rule ent_refl
+
+method keep_drop = 
+  rule keep_drop_init, ((rule keep_drop_step)+; fail), keep_drop_simp, keep_drop_simp
+
+
+
+lemma hnr_let[hnr_rule]:
   assumes 
     "hnr \<Gamma> vi \<Gamma>\<^sub>1 R\<^sub>1 v" 
-    "\<And>xi x. hnr (\<Gamma>\<^sub>1 * R\<^sub>1 x xi) (fi xi) \<Gamma>' R (f x)"
+    "\<And>xi x. hnr (\<Gamma>\<^sub>1 * R\<^sub>1 x xi) (fi xi) (\<Gamma>' x xi) R (f x)"
+    "\<And>xi x. keep_drop (\<Gamma>' x xi) \<Gamma>'' (R\<^sub>1' x xi)"
   shows 
-    "hnr \<Gamma> (do { x \<leftarrow> vi; fi x }) \<Gamma>' R (let x = v in f x)"
-  supply[sep_heap_rules] = assms[THEN hnrD]
+    "hnr \<Gamma> (do { x \<leftarrow> vi; fi x }) \<Gamma>'' R (let x = v in f x)"
+  supply[sep_heap_rules] = assms(1, 2)[THEN hnrD]
   apply(rule hnrI)
+  apply sep_auto
+  apply(sep_drule r: assms(3)[unfolded keep_drop_def])
   by sep_auto
 
 lemma hnr_if: 
@@ -59,7 +103,7 @@ shows
   sorry *)
 
 
-lemma hnr_array_nth: "
+lemma hnr_array_nth [hnr_rule, hnr_rule_2]: "
     hnr
      (xsi \<mapsto>\<^sub>a xs * id_assn i ii)
      (array_nth_safe xsi ii) 
@@ -70,7 +114,7 @@ lemma hnr_array_nth: "
   apply(rule hnrI)
   by sep_auto
 
-lemma hnr_array_update: "
+lemma hnr_array_update [hnr_rule, hnr_rule_2]: "
     hnr 
       (xsi \<mapsto>\<^sub>a xs * id_assn i ii * id_assn v vi) 
       (array_update_safe ii vi xsi) 
@@ -86,17 +130,21 @@ lemma hnr_pass: "hnr (id_assn x xi) (return xi) emp id_assn x"
   apply(rule hnrI)
   by sep_auto
 
-(* TODO : *)
+lemma hnr_copy: "hnr (id_assn x xi) (return xi) (id_assn x xi) id_assn x"
+  unfolding id_assn_def
+  apply(rule hnrI)
+  by sep_auto
+
 lemma hnr_frame:
   assumes
-    "hnr \<Gamma> fi \<Gamma>' R f"
     "\<Gamma>\<^sub>P \<Longrightarrow>\<^sub>A \<Gamma> * F"
+    "hnr \<Gamma> fi \<Gamma>' R f"
   shows
     "hnr \<Gamma>\<^sub>P fi (\<Gamma>' * F) R f"
   apply(rule hnrI)
   by (smt (verit) assms(1) assms(2) assn_aci(10) fi_rule hnrD hoare_triple_def)
 
-lemma hnr_lookup: "
+lemma hnr_lookup[hnr_rule_diff_arr]: "
   hnr
     (master_assn t * id_assn i ii * \<up>(t \<turnstile> xs \<sim> xsi \<and> i < length xs))
     (lookup xsi ii)
@@ -119,6 +167,12 @@ lemma hnr_realize: "
   using realize[of t xs xsi]
   by(sep_auto simp: cons_post_rule ent_refl_true)
 
+lemma ht_combine_post: "<P> c <Q> \<Longrightarrow> <P> c <Q'> \<Longrightarrow> <P> c <\<lambda>r. Q r \<and>\<^sub>A Q' r>"
+  unfolding hoare_triple_def
+  by(auto simp: Let_def mod_and_dist)
+
+thm ht_combine_post[OF update update', simplified]
+
 lemma hnr_update: "
   hnr
     (master_assn t * \<up>(t \<turnstile> xs \<sim> xsi \<and> i < length xs) * id_assn i ii * id_assn v vi)
@@ -131,16 +185,46 @@ lemma hnr_update: "
   using update[of t xs xsi i v]
   by sep_auto
 
-lemma hnr_update': "
+lemma hnr_update'[hnr_rule_diff_arr]: "
   hnr
     (master_assn t * \<up>(t \<turnstile> xs \<sim> xsi \<and> i < length xs) * id_assn i ii * id_assn v vi)
     (update xsi ii vi)
     (id_assn i ii * id_assn v vi)
-    (\<lambda>_ _. \<exists>\<^sub>At'. master_assn t' * \<up>(\<forall>xs' xsi'. t \<turnstile> xs' \<sim>  xsi' \<longrightarrow> t' \<turnstile> xs' \<sim>  xsi'))
+    (\<lambda>xs xsi. \<exists>\<^sub>At'. master_assn t' * \<up>((\<forall>xs' xsi'. t \<turnstile> xs' \<sim>  xsi' \<longrightarrow> t' \<turnstile> xs' \<sim>  xsi') \<and> t' \<turnstile> xs \<sim> xsi))
     (xs [i:= v])"
   unfolding id_assn_def
   apply(rule hnrI)
-  using update'[of t xs xsi i v]
+  apply(sep_auto)
+  apply(rule cons_post_rule)
+   apply(rule fi_rule[OF update''])
+  apply solve_entails
   by sep_auto
+
+(* lemma hnr_array_update [hnr_rule, hnr_rule_2]: "
+    hnr 
+      (xsi \<mapsto>\<^sub>a xs * id_assn i ii * id_assn v vi) 
+      (array_update_safe ii vi xsi) 
+      (id_assn i ii * id_assn v vi) 
+      array_assn 
+      (xs [i:= v])"
+  unfolding id_assn_def
+  apply(rule hnrI)
+  by sep_auto *)
+
+lemma hnr_update_2[hnr_rule_diff_arr]: "
+  hnr
+    (id_assn i ii * id_assn v vi)
+    (update xsi ii vi)
+    (id_assn i ii * id_assn v vi)
+    (\<lambda>xs xsi. \<exists>\<^sub>At'. master_assn t' * \<up>((\<forall>xs' xsi'. t \<turnstile> xs' \<sim>  xsi' \<longrightarrow> t' \<turnstile> xs' \<sim>  xsi') \<and> t' \<turnstile> xs \<sim> xsi))
+    (xs [i:= v])"
+  unfolding id_assn_def
+  apply(rule hnrI)
+  apply(sep_auto)
+  apply(rule cons_post_rule)
+   apply(rule fi_rule[OF update''])
+   apply solve_entails
+     apply sep_auto
+  sorry
 
 end
