Test.thy
@@ -28,19 +28,71 @@ value "(xs[1 := 2], xs[1 := 3])"
 
 definition test1 where
   "test1 xs = 
-    (let c1 = 1; c2 = 2; c3 = 3; t1 = xs[c1 := c2]; t2 = t1[c1 := c3]; t3 = t2 ! c2 in t3)"
+    (let c1 = (let x = 1 in x); c2 = 2; c3 = 3; t1 = xs[c1 := c2]; t2 = t1[c1 := c3]; t3 = t2 ! c2 in t3)"
+
+attribute_setup framed =
+    \<open>Scan.succeed (Thm.rule_attribute [] (fn _ => fn thm => @{thm hnr_frame} OF [asm_rl, thm]))\<close>
+    \<open>Add frame to hnr rule\<close>
+
+thm hnr_rule[framed]
+
+method hnr_rule = 
+  (rule hnr_rule[framed] hnr_copy[framed] hnr_return[framed], (frame_inference; fail))
+
+method hnr_rule_2 = 
+  (rule hnr_rule_2[framed] hnr_copy[framed], (frame_inference; fail)) | (rule hnr_let hnr_return)
+
+method hnr_rule_diff_arr =
+  (rule hnr_rule_diff_arr[framed] hnr_copy[framed], (frame_inference; fail)) | (rule hnr_let hnr_return)
+
+method hnr = (hnr_rule | keep_drop)+
+
+method hnr_2 = (hnr_rule_2 | keep_drop)+
+
+method hnr_diff_arr = (hnr_rule_diff_arr | keep_drop)+
+
+schematic_goal "hnr (array_assn xs xsi) (?c :: ?'a Heap) ?\<Gamma>' ?R (test1 xs)"
+  by hnr_2
 
 schematic_goal "hnr (array_assn xs xsi) (?c :: ?'a Heap) ?\<Gamma>' ?R (test1 xs)"
   unfolding test1_def 
-  apply(rule hnr_let hnr_return)+
-  apply(rule hnr_frame[OF hnr_array_update], frame_inference)
   apply(rule hnr_let)
-  apply(rule hnr_frame[OF hnr_array_update], frame_inference)
   apply(rule hnr_let)
-  apply(rule hnr_frame[OF hnr_array_nth], frame_inference)
-  apply(rule hnr_frame[OF hnr_pass])
+  apply(rule hnr_return)
+  apply(rule hnr_copy[framed], frame_inference)
+  apply keep_drop
+     (* Here: *)
+   (* apply(rule hnr_let[framed])
+  apply(frame_inference) *)
+  apply(rule hnr_let)
+  apply(rule hnr_return)
+  apply(rule hnr_let)
+  apply(rule hnr_return)
+  apply(rule hnr_let)
+  apply(rule hnr_array_update[framed], frame_inference)
+  apply(rule hnr_let)
+  apply(rule hnr_array_update[framed], frame_inference)
+  apply(rule hnr_let)
+  apply(rule hnr_array_nth[framed], frame_inference)
+  apply(rule hnr_copy[framed], frame_inference)
+  by keep_drop+
+
+schematic_goal "hnr (array_assn xs xsi) (?c :: ?'a Heap) ?\<Gamma>' ?R (test1 xs)"
+  unfolding test1_def 
+  apply(hnr_rule_diff_arr)
+    apply(hnr_rule_diff_arr)
+      apply(hnr_rule_diff_arr)
+     apply(hnr_rule_diff_arr)
+  apply keep_drop
+   apply(hnr_rule_diff_arr)
+     apply(hnr_rule_diff_arr)
+    apply(hnr_rule_diff_arr)
+      apply(hnr_rule_diff_arr)
+     apply(hnr_rule_diff_arr)
+  (* How to get to master_assn in the first place? *)
+       apply(rule hnr_update'[framed])
   sorry
-  
+
 export_code array_nth_safe array_update_safe in SML_imp
 
 end
